init Ax

spec_streebog_xlps.v
@@ -5,6 +5,8 @@ Require Import compcert.lib.Zbits.
 #[export] Instance CompSpecs : compspecs. make_compspecs prog. Defined.
 Definition Vprog : varspecs. mk_varspecs prog. Defined.
 Require Import functional_spec.
+Require Import spec_streebog_xor.
+
 
 Import ListNotations.
 
@@ -22,6 +24,11 @@ Definition Ax_to_vals (a : list (list int64)) : list (list val) :=
   map (fun i => map (fun j => Vlong j) i) a.
 
 
+Definition r_i_expr (i : Z) (j : Z) (x_content y_content : block512) : val :=
+  Vlong (Int64.repr (Znth j (block512_to_chunks (Vec512.xor x_content y_content)))).
+
+
+
 Definition gen_Ax : list (list int64) :=
   map (fun i =>
          map (fun j =>
@@ -29,88 +36,184 @@ Definition gen_Ax : list (list int64) :=
              (seq 0 256))
       (seq 0 8).
 
+
+(* Definition Spec_streebog_xlps_VarSpecs : varspecs := (_Ax, (tarray (tarray tulong 256) 8))::nil. *)
+
 Definition streebog_xlps_spec :=
   DECLARE _streebog_xlps
   WITH sh_r : share, sh_w : share,
-       x : val, y : val, z : val,
-       x_content : block512, y_content : block512, z_content : block512,
-       Ax : val
+       x : val, y : val, data : val,
+       x_content : block512, y_content : block512, data_content : block512,
+       gv : globals
   PRE [tptr tuint512, tptr tuint512, tptr tuint512]
     PROP(readable_share sh_r; writable_share sh_w)
-    PARAMS (x; y; z)
+    PARAMS (x; y; data)
+    (* LOCAL (gvars gv) *)
     SEP (data_at sh_r tuint512 (block512_to_vals x_content) x;
          data_at sh_r tuint512 (block512_to_vals y_content) y;
-         data_at sh_w tuint512 (block512_to_vals z_content) z;
-         data_at sh_r (tarray (tarray tulong 256) 8) (Ax_to_vals gen_Ax) Ax)
+         data_at sh_w tuint512 (block512_to_vals data_content) data;
+         data_at sh_r (tarray (tarray tulong 256) 8) (Ax_to_vals gen_Ax) (gv _Ax))
   POST [tvoid]
     PROP()
+    (* LOCAL (gvars gv) *)
     RETURN()
     SEP (data_at sh_r tuint512 (block512_to_vals x_content) x;
          data_at sh_r tuint512 (block512_to_vals y_content) y;
-         data_at sh_w tuint512 (block512_to_vals (LPSX x_content y_content)) z;
-         data_at sh_r (tarray (tarray tulong 256) 8) (Ax_to_vals gen_Ax) Ax).
+         data_at sh_w tuint512 (block512_to_vals (LPSX x_content y_content)) data;
+         data_at sh_r (tarray (tarray tulong 256) 8) (Ax_to_vals gen_Ax) (gv _Ax)).
 
 
 Definition inv_data_mem (sh :share) (x : val) (x_content : block512) : mpred :=
   data_at sh tuint512 (block512_to_vals x_content) x.
 
-Definition inv_data_mem_res (sh :share) (i : Z) (z : val) (x_content y_content z_content : block512) : mpred :=
+Definition inv_data_mem_res (sh :share) (i : Z) (z : val) (x_content y_content data_content : block512) : mpred :=
   (
    data_at sh tuint512 (
       (sublist 0 i (block512_to_vals (LPSX x_content y_content)) ++
-                            (sublist i 8 (block512_to_vals z_content)))) z).
+                            (sublist i 8 (block512_to_vals data_content)))) z).
 
-(*
-Definition A_rev := rev A.
 
-Fixpoint calc_a (A : list int64) (t : Z) (i : nat) (a : int64): int64 :=
-  match i with
-  | O => a
-  | S i' => match A with
-    | [] => a
-    | x :: xs => let x' := Z_mod_two_p t 1 * x
-      in calc_a xs (Z.shiftr 1 t) i' (Int64.xor a x)
-    end
+
+Fixpoint Z_to_xor_list (k : nat) (x y : Z) : list val :=
+  match k with
+  | O => Vlong (Int64.xor (Int64.repr (LSB 64 x)) (Int64.repr (LSB 64 y))) :: nil
+  | S k' => Vlong (Int64.xor (Int64.repr (LSB 64 x)) (Int64.repr (LSB 64 y))) ::
+            (Z_to_xor_list k' (Z.shiftr x (Z.of_nat 64)) (Z.shiftr y (Z.of_nat 64)))
   end.
 
-Fixpoint create_Ax (pi : list byte) (A : list int64) (i : Z) : list int64 :=
-  match i with
-  | O => []
-  | S i' =>
-    match pi with
-    | [] => []
-    | x :: xs =>
-    end
-  end.
+Lemma r_i_eq : forall (i j : Z) (r1 r2 : block512),
+  Zlength (block512_to_chunks r1) = 8 -> Zlength (block512_to_chunks r2) = 8 ->
+  r_i_expr i j r1 r2 = Znth j (Z_to_xor_list 8 (Vec512.unsigned r1) (Vec512.unsigned r2)).
+Proof.
+  intros i j r1 r2 H1 H2.
+  (* intros i j r1 r2. *)
+  unfold r_i_expr.
+  unfold Z_to_xor_list.
+  rewrite !Z.shiftr_shiftr.
+  unfold block512_to_chunks.
+  unfold Z_to_chunks.
+  rewrite !xor_repr_comm.
+  rewrite !xor_LSB_comm.
+  Search (Z.lxor).
+  rewrite <- !Z.shiftr_lxor.
+  rewrite !Z.shiftr_shiftr.
+  Search (Znth).
+  Search map.
+  (* induction j as [|j' Hj']. *)
+  (* - simpl. *)
+  (*   unfold block512_to_chunks in *. *)
+  (*   unfold Z_to_chunks in *. *)
+  (*   rewrite Znth_0_cons. *)
+  (*   induction i as [|i' Hi']. *)
+  (*   + rewrite Znth_0_cons. *)
+  (*     rewrite Z.shiftr_0_r. *)
+  (*     rewrite xor_repr_comm. *)
+  (*     rewrite xor_LSB_comm. *)
+  (*     rewrite xor_unsigned_comm. *)
+  (*     reflexivity. *)
+  (*   + rewrite Nat2Z.inj_succ.  *)
+  (*     Search Zlength. *)
+  (*     Search (Znth). *)
+  (* unfold Z_to_xor_list. *)
+  (* unfold block512_to_chunks, Z_to_chunks. *)
+  (* rewrite Z.shiftr_0_r. *)
 
-Fixpoint create_Ax (pi : list byte) (A : list int64) : list (list int64) . *)
+  (* split. *)
+  (* +  *)
+  (*   rewrite xor_repr_comm. *)
+  (*   rewrite xor_LSB_comm. *)
+  (*   rewrite xor_unsigned_comm. *)
+  (*   unfold block512_to_chunks, Z_to_chunks. *)
+  (*   rewrite Znth_0_cons. *)
+  (*   reflexivity. *)
+Admitted.
 
-
+Definition inv_data_mem2 (sh :share) (x : val) : mpred :=
+  data_at_ sh tuint512 x.
 
 
 Lemma body_streebog_xlps :
-  semax_body Vprog [] f_streebog_xlps streebog_xlps_spec.
+  semax_body  Vprog [] f_streebog_xlps streebog_xlps_spec.
 Proof.
   start_function.
-  assert (Zlength (block512_to_int64s x_content) = 8) by reflexivity.
-  assert (Zlength (block512_to_int64s y_content) = 8) by reflexivity.
-  assert (Zlength (block512_to_int64s z_content) = 8) by reflexivity.
+
+  (* assert (Zlength (block512_to_chunks x_content) = 8) by reflexivity.
+  assert (Zlength (block512_to_chunks y_content) = 8) by reflexivity. *)
+  (* assert (Zlength (block512_to_int64s z_content) = 8) by reflexivity. *)
 
   do 24 forward.
+
+  Definition Ax_vals := Ax_to_vals gen_Ax.
 
   deadvars!.
   forward_loop
    (EX i:Z,(*EX j:Z, EX data: list int64,*) 
-    PROP(0 <= i <= 7)
-    LOCAL (temp _i (Vint (Int.repr i)))
+    PROP(0 <= i <= 7;
+          sublist 0 i (block512_to_vals (LPSX x_content y_content)) =
+          sublist 0 i (block512_to_vals data_content))
+    LOCAL (temp _i (Vint (Int.repr i));
+            temp _r0 (r_i_expr i 0 x_content y_content);
+            temp _r1 (r_i_expr i 1 x_content y_content);
+            temp _r2 (r_i_expr i 2 x_content y_content);
+            temp _r3 (r_i_expr i 3 x_content y_content);
+            temp _r4 (r_i_expr i 4 x_content y_content);
+            temp _r5 (r_i_expr i 5 x_content y_content);
+            temp _r6 (r_i_expr i 6 x_content y_content);
+            temp _r7 (r_i_expr i 7 x_content y_content);
+            gvars gv;
+            temp _data data) 
     SEP (inv_data_mem sh_r x x_content; inv_data_mem sh_r y y_content; 
-         inv_data_mem_res sh_w i z x_content y_content z_content;
-         data_at sh_r (tarray (tarray tulong 256) 8) (Ax_to_vals gen_Ax) Ax)
+         (* inv_data_mem sh_w data data_content;  *)
+          data_at_ sh_w tuint512 data;
+         (* inv_data_mem_res sh_w i data x_content y_content data_content; *)
+         data_at sh_r (tarray (tarray tulong 256) 8) Ax_vals (gv _Ax))
     ).
   - forward.
     entailer!.
     Exists 0. 
-    entailer!. 
+    entailer!.
+    split. 
+    + rewrite r_i_eq; reflexivity.
+    + split.  
+      ++ now rewrite r_i_eq.
+      ++ split.
+        +++ now rewrite r_i_eq.
+        +++ split. 
+          ++++ now rewrite r_i_eq.
+          ++++ split.
+            +++++ now rewrite r_i_eq.
+            +++++ split.
+              ++++++ now rewrite r_i_eq.
+              ++++++ split.
+                +++++++ now rewrite r_i_eq.
+                +++++++ split.  now rewrite r_i_eq. admit.
+    - Intros i. forward_if.
+      -- abbreviate_semax. forward.
+        * entailer!. admit.
+        * entailer!. (*rewrite Znth_0_cons.*) admit. 
+        * forward. deadvars!. forward.
+          ** entailer!. admit.
+          ** admit.
+      -- lia.
+         
+
+    (* + rewrite r_i_eq; reflexivity.
+    + split.
+      ++ rewrite r_i_eq.
+        +++  unfold Z_to_xor_list. rewrite Znth_pos_cons.
+          ++++ rewrite Znth_0_cons. reflexivity.
+          ++++ lia.
+        +++ reflexivity.
+        +++ reflexivity.
+      ++ split.
+        *** now rewrite r_i_eq.
+        *** split.
+            **** now rewrite r_i_eq.
+            **** split.
+      lia. reflexivity. reflexivity. rewrite Znth_pos_cons. rewrite Znth_pos_cons. rewrite Znth_0_cons.
+      split. reflexivity. 
+
+    + reflexivity.
   - hint. Intros i. hint.
     forward_if.
     + hint. abbreviate_semax. unfold Ax_to_vals. forward.
@@ -123,6 +226,6 @@ Proof.
     hint.
     lia .
     hint.
-  - hint.
+  - hint. *)
 
 Qed.
